acyclicity proof of ast-to-cfg transformation without break: one subcase missing

AstToCfg_simple.dfy
@@ -17,7 +17,7 @@ module AstToCfg {
     match c
     case SimpleCmd(_) => true
     case Break(optLbl) => false
-    case Seq(c1, c2) => NoBreaksScopesLoops(c1) && NoBreaksScopesLoops(c2)
+    case Seq(thn, els) => NoBreaksScopesLoops(thn) && NoBreaksScopesLoops(els)
     case Loop(_,_) => false
     case Scope(_,_,_) => false
     case If(_, thn, els) => NoBreaksScopesLoops(thn) && NoBreaksScopesLoops(els)
@@ -33,6 +33,11 @@ module AstToCfg {
       assert (s - {x}) + {x} == s;
       Math.Max(subRes, x)
   }
+
+  /*
+  lemma Test(a: nat, b: nat, c: nat, s1: set<nat>, s2: set<nat>, s3: set<nat>)
+    ensures CoveredSet(a, b, s1, s2) + CoveredSet(b, c, s2, )
+  */
 
   /** 
     Transforms the Ast `c` into a Cfg.
@@ -51,66 +56,101 @@ module AstToCfg {
     precedingBlock: (BlockId, BasicBlock), 
     nextVersion: BlockId) : (Option<Cfg>, BlockId, Option<(BlockId, BasicBlock)>) //Option for exit block needed once break statements are taken into account
     requires NoBreaksScopesLoops(c)
-    ensures (var res := AstToCfgAux(c, precedingBlock, nextVersion); 
-             res.2 != None && (if res.0 == None then nextVersion == res.1 else nextVersion <= res.1))
+    requires precedingBlock.0 < nextVersion
+    ensures  var res := AstToCfgAux(c, precedingBlock, nextVersion); 
+             var exitBlockOpt := res.2;
+             var nextVersion' := res.1;
+             && (exitBlockOpt != None)
+             && (if res.0 == None then 
+                    && nextVersion == nextVersion' 
+                    && precedingBlock.0 == exitBlockOpt.value.0 
+                 else 
+                  && nextVersion < nextVersion' 
+                  && (nextVersion <= exitBlockOpt.value.0 < nextVersion')
+                  && res.0.value.successors.Keys <= CoveringSet(nextVersion, nextVersion', {precedingBlock.0}, {exitBlockOpt.value.0})
+                )
   {
     match c
     case SimpleCmd(simpleC) => (None, nextVersion, Some((precedingBlock.0, precedingBlock.1+[simpleC])))
-    case Seq(c1, c2) =>
-      var (optCfg1, nextVersion1, optExit1) := AstToCfgAux(c1, precedingBlock, nextVersion);
+    case Seq(thn, els) =>
+      var (optCfg1, nextVersion1, optExit1) := AstToCfgAux(thn, precedingBlock, nextVersion);
 
       if optExit1.None? then
-        //c2 will never be reached
+        //els will never be reached
         (optCfg1, nextVersion1, optExit1)
       else
-        var (optCfg2, nextVersion2, optExit2) := AstToCfgAux(c2, optExit1.value, nextVersion1);
+        var (optCfg2, nextVersion2, optExit2) := AstToCfgAux(els, optExit1.value, nextVersion1);
 
         if optCfg1.None? then
-          //since the exit block for c1 becomes the preceding block for c2, we can take the result for c2
+          //since the exit block for thn becomes the preceding block for els, we can take the result for els
+          assert optCfg2.Some? ==> nextVersion == nextVersion1 && optExit1.value.0 == precedingBlock.0;
           (optCfg2, nextVersion2, optExit2)
         else if optCfg2.None? then
+          var cfg1 := optCfg1.value;
+          assert optExit2.value.0 == optExit1.value.0;
+          assert nextVersion1 == nextVersion2;
           (optCfg1, nextVersion2, optExit2)
         else
           //merge cfgs
           var cfg1 := optCfg1.value;
           var cfg2 := optCfg2.value;
+
+          var cover1 := CoveringSet(nextVersion, nextVersion1, {precedingBlock.0}, {optExit1.value.0});
+          var cover2 := CoveringSet(nextVersion1, nextVersion2, {optExit1.value.0}, {optExit2.value.0});
+          var cover3 := CoveringSet(nextVersion, nextVersion2, {precedingBlock.0}, {optExit2.value.0});
+          assert cover1 + cover2 <= cover3;
+
           (Some(Cfg(cfg1.entry, cfg1.blocks + cfg2.blocks, cfg1.successors + cfg2.successors)), nextVersion2, optExit2)
-    case If(optCond, c1, c2) => 
-      var (c1StartId, c1StartBlock) := if optCond.Some? then (nextVersion, [Assume(optCond.value)]) else (nextVersion, []);
-      var (c2StartId, c2StartBlock) := if optCond.Some? then (nextVersion+1, [Assume(UnOp(Not, optCond.value))]) else (nextVersion+1, []);
+    case If(optCond, thn, els) => 
+      /** CFG thn branch */
+      var (thnStartId, thnStartBlock) := if optCond.Some? then (nextVersion, [Assume(optCond.value)]) else (nextVersion, []);
+      var (optCfg1, nextVersion1, optExit1) := AstToCfgAux(thn, (thnStartId, thnStartBlock), nextVersion+1);
 
-      var (optCfg1, nextVersion1, optExit1) := AstToCfgAux(c1, (c1StartId, c1StartBlock), nextVersion);
-
-      var (optCfg2, nextVersion2, optExit2) := AstToCfgAux(c2, (c2StartId, c2StartBlock), nextVersion1);
-
-      var (entryBlockId, entryBlock) := precedingBlock;
+      /** CFG els branch */
+      var (elsStartId, elsStartBlock) := if optCond.Some? then (nextVersion1, [Assume(UnOp(Not, optCond.value))]) else (nextVersion1, []);
+      var (optCfg2, nextVersion2, optExit2) := AstToCfgAux(els, (elsStartId, elsStartBlock), nextVersion1+1);
 
       /** 
         * precedingBlock is the entry block 
-        * connect precedingBlock to c1StartId and c2StartId
+        * connect precedingBlock to thnStartId and elsStartId
         * if then/else branch have active exit blocks, then connect those to a fresh basic block, which will became the active basic block
       */
+      var (entryBlockId, entryBlock) := precedingBlock;
 
-      var successors1 := if optCfg1.Some? then optCfg1.value.successors else map[];
-      var successors2 := if optCfg2.Some? then successors1 + optCfg2.value.successors else successors1;
-      var successors3 := successors2[entryBlockId := [c1StartId, c2StartId]];
+      /** new successor relation */
+      var (blocksThnEls, successorsThnEls) := 
+        if optCfg1.Some? && optCfg2.Some? then
+          (optCfg1.value.blocks + optCfg2.value.blocks, optCfg1.value.successors + optCfg2.value.successors)
+        else if optCfg1.Some? then
+          (optCfg1.value.blocks, optCfg1.value.successors)
+        else if optCfg2.Some? then
+          (optCfg2.value.blocks, optCfg2.value.successors)
+        else
+          (map[], map[]);
 
-      var blocks1 := if optCfg1.Some? then optCfg1.value.blocks else map[];
-      var blocks2 := if optCfg2.Some? then blocks1 + optCfg2.value.blocks else blocks1;
-      var blocks3 := blocks2[entryBlockId := entryBlock];
+      var blocksBeforeJoin := blocksThnEls[entryBlockId := entryBlock]; 
+      var successorsBeforeJoin := successorsThnEls[entryBlockId := [thnStartId, elsStartId]];
 
       if optExit1.Some? && optExit2.Some? then
         //connect the end of both branches to a new block
         var (joinId, joinBlock) := (nextVersion2, []);
-        var (thenExitId, thenExitBlock) := optExit1.value;
-        var (elseExitId, elseExitBlock) := optExit2.value;
-        var successors4 := successors3[thenExitId := [joinId]][elseExitId := [joinId]];
-        var cfg := Cfg(entryBlockId, blocks3, successors3[thenExitId := [joinId]][elseExitId := [joinId]]);
+        var (thnExitId, thenExitBlock) := optExit1.value;
+        var (elsExitId, elseExitBlock) := optExit2.value;
+
+        var blocks := blocksBeforeJoin[thnExitId := thenExitBlock];
+        var successors := successorsBeforeJoin[thnExitId := [joinId]][elsExitId := [joinId]];
+        var cfg := Cfg(entryBlockId, blocks, successors);
+
         (Some(cfg), nextVersion2+1, Some((joinId, joinBlock)))
       else 
-        var cfg := Cfg(entryBlockId, blocks3, successors3);
+        var cfg := Cfg(entryBlockId, blocksBeforeJoin, successorsBeforeJoin);
         var optExitResult := if optExit1.Some? then optExit1 else optExit2;
         (Some(cfg), nextVersion2, optExitResult)
+  }
+
+  function CoveringSet(oldVersion: nat, newVersion: nat, including: set<nat>, excluding: set<nat>) : set<nat>
+  {
+    ((set x : nat | oldVersion <= x < newVersion) + including) - excluding
   }
 
   lemma AstToCfgAcyclic(
@@ -118,6 +158,7 @@ module AstToCfg {
     precedingBlock: (BlockId, BasicBlock), 
     nextVersion: BlockId)
     requires NoBreaksScopesLoops(c)
+    requires precedingBlock.0 < nextVersion
     ensures  
       var res := AstToCfgAux(c, precedingBlock, nextVersion); 
       var nextVersion' := res.1;
@@ -125,65 +166,137 @@ module AstToCfg {
 
       if res.0.Some? then  
         var cfg := res.0.value;
-        //TODO: 
-        /*
-        cfg.entry in cfg.blocks.Keys &&
-        cfg.blocks.Keys == cfg.successors.Keys &&
-        */
-        cfg.entry == precedingBlock.0 &&
-        IsAcyclicAlt(cfg, cfg.entry, set x : nat | nextVersion <= x < nextVersion')
+        var s := cfg.successors;
+        
+        && cfg.entry == precedingBlock.0
+        && (forall n :: n in s.Keys ==>   
+            (forall i :: 0 <= i < |s[n]| ==> (s[n][i] == exitBlockId || s[n][i] in s.Keys))) 
+        && cfg.entry in s.Keys 
+        && IsAcyclicAlt(cfg.successors, cfg.entry, CoveringSet(nextVersion, nextVersion', {precedingBlock.0}, {exitBlockId}))
+
       else  
         precedingBlock.0 == exitBlockId 
         //TODO: && precedingBlock.1 <= exitBlock
   {
     match c {
       case SimpleCmd(_) => 
-      case Seq(c1, c2) =>
-        var (optCfg1, nextVersion1, optExit1) := AstToCfgAux(c1, precedingBlock, nextVersion);
+      case Seq(thn, els) =>
+        var (optCfg1, nextVersion1, optExit1) := AstToCfgAux(thn, precedingBlock, nextVersion);
 
         if optExit1.None? {
-          //c2 will never be reached
+          //els will never be reached
           //this case cannot occur in the simplified setting
           assert false;
         } else {
-          var (optCfg2, nextVersion2, optExit2) := AstToCfgAux(c2, optExit1.value, nextVersion1);
-          AstToCfgAcyclic(c2, optExit1.value, nextVersion2);
+          var (optCfg2, nextVersion2, optExit2) := AstToCfgAux(els, optExit1.value, nextVersion1);
+          AstToCfgAcyclic(els, optExit1.value, nextVersion2);
 
           var (exitBlockId2, exitBlock2) := optExit2.value;
 
           if optCfg1.None? {
-            //since the exit block for c1 becomes the preceding block for c2, we can take the result for c2
+            //since the exit block for thn becomes the preceding block for els, we can take the result for els
             //(optCfg2, nextVersion2, optExit2)
             if optCfg2.Some? {
               var cfg2 := optCfg2.value;
               
-              IsAcyclicLargerCover(cfg2, cfg2.entry, set x : nat | nextVersion1 <= x < nextVersion2, set x : nat | nextVersion <= x < nextVersion2);
+              IsAcyclicLargerCover(
+                cfg2.successors, 
+                cfg2.entry, 
+                CoveringSet(nextVersion1, nextVersion2, {optExit1.value.0}, {exitBlockId2}), 
+                CoveringSet(nextVersion, nextVersion2, {optExit1.value.0}, {exitBlockId2})
+              );
             }
           } else if optCfg2.None? {
             //(optCfg1, nextVersion2, optExit2)
           } else {
-
-            /** precondition of merge lemma  
-                requires cover1 !! cover2
-                requires r1.Keys !! r2.Keys
-                requires IsAcyclicAlt(r1, n1Entry, cover1)
-                requires IsAcyclicAlt(r2, n2Entry, cover2)
-
-                requires n1Entry in r1.Keys || n1Entry == n2Entry
-                requires !(n2Entry in r1.Keys)
-            */
-
-            assume false;
             //merge cfgs
             var cfg1 := optCfg1.value;
             var cfg2 := optCfg2.value;
 
-            assume false;
-            //assert cfg1.successors.Keys !! cfg2.successors.Keys;
-            //(Some(Cfg(cfg1.entry, cfg1.blocks + cfg2.blocks, cfg1.successors + cfg2.successors)), nextVersion2, optExit2)
+            var cover1 := CoveringSet(nextVersion, nextVersion1, {precedingBlock.0}, {cfg2.entry});
+            var cover2 := CoveringSet(nextVersion1, nextVersion2, {cfg2.entry}, {exitBlockId2});
+            var cover3 := CoveringSet(nextVersion, nextVersion2, {precedingBlock.0}, {exitBlockId2});
+
+            assert cover1 !! cover2;
+            assert cfg1.successors.Keys !! cfg2.successors.Keys;
+
+            IsAcyclicMerge(
+              cfg1.successors, cfg2.successors, cfg1.entry, cfg2.entry, 
+              cover1,
+              cover2
+              );
+
+            IsAcyclicLargerCover(cfg1.successors + cfg2.successors, cfg1.entry, cover1 + cover2, cover3);
           }
         }
-      case _ => assume false;
+      case If(optCond, thn, els) => 
+        var (thnStartId, thnStartBlock) := if optCond.Some? then (nextVersion, [Assume(optCond.value)]) else (nextVersion, []);
+        var (optCfg1, nextVersion1, optExit1) := AstToCfgAux(thn, (thnStartId, thnStartBlock), nextVersion+1);
+
+        var (elsStartId, elsStartBlock) := if optCond.Some? then (nextVersion1, [Assume(UnOp(Not, optCond.value))]) else (nextVersion1, []);
+        var (optCfg2, nextVersion2, optExit2) := AstToCfgAux(els, (elsStartId, elsStartBlock), nextVersion1+1);
+
+        if optCfg1.Some? && optCfg2.Some? {
+          var cfg1 := optCfg1.value;
+          var cfg2 := optCfg2.value;
+          var exit1 := optExit1.value;
+          var exit2 := optExit2.value;
+          var s1 := cfg1.successors;
+          var s2 := cfg2.successors;
+
+          var cover1 := CoveringSet(nextVersion+1, nextVersion1, {nextVersion}, {exit1.0});
+          assert IsAcyclicAlt(s1, cfg1.entry, cover1);
+
+          var cover2 := CoveringSet(nextVersion1+1, nextVersion2, {nextVersion1}, {exit2.0});
+          assert IsAcyclicAlt(s2, cfg2.entry, cover2);
+
+          IsAcyclicExtend2(s1, s2, cfg1.entry, cover1);
+          IsAcyclicLargerCover(s1 + s2, cfg1.entry, cover1, cover1+cover2);
+          assert IsAcyclicAlt(s1 + s2, cfg1.entry, cover1+cover2);
+
+          IsAcyclicExtend(s1, s2, cfg2.entry, cover2);
+          IsAcyclicLargerCover(s1 + s2, cfg2.entry, cover2, cover1+cover2);
+          assert IsAcyclicAlt(s1 + s2, cfg2.entry, cover1+cover2);
+
+          var (entryBlockId, entryBlock) := precedingBlock;
+
+          var successorsBeforeJoin := (s1 + s2)[entryBlockId := [thnStartId, elsStartId]];
+
+          assert IsAcyclicAlt(successorsBeforeJoin, entryBlockId, cover1+cover2+{entryBlockId}) by {
+            calc {
+              IsAcyclicAlt(successorsBeforeJoin, entryBlockId, cover1+cover2+{entryBlockId});
+              IsAcyclicSeqAlt(successorsBeforeJoin, [thnStartId, elsStartId], cover1+cover2);
+              IsAcyclicAlt(successorsBeforeJoin, thnStartId, cover1+cover2) &&
+              IsAcyclicSeqAlt(successorsBeforeJoin, [elsStartId], cover1+cover2);
+              IsAcyclicAlt(successorsBeforeJoin, thnStartId, cover1+cover2) &&
+              IsAcyclicAlt(successorsBeforeJoin, elsStartId, cover1+cover2);
+              { IsAcyclicUpdate(s1+s2, cfg1.entry, entryBlockId, [thnStartId, elsStartId], cover1+cover2);
+                IsAcyclicUpdate(s1+s2, cfg2.entry, entryBlockId, [thnStartId, elsStartId], cover1+cover2);
+              }
+              IsAcyclicAlt(s1+s2, thnStartId, cover1+cover2) &&
+              IsAcyclicAlt(s1+s2, elsStartId, cover1+cover2);
+            }
+          }
+
+          var (thnExitId, thenExitBlock) := optExit1.value;
+          var (elsExitId, elseExitBlock) := optExit2.value;
+
+          IsAcyclicUpdate2(successorsBeforeJoin, entryBlockId, thnExitId, [nextVersion2], cover1+cover2+{entryBlockId});
+          IsAcyclicUpdate2(successorsBeforeJoin[thnExitId := [nextVersion2]], entryBlockId, elsExitId, [nextVersion2], cover1+cover2+{entryBlockId}+{thnExitId});
+
+          var successors := successorsBeforeJoin[thnExitId := [nextVersion2]][elsExitId := [nextVersion2]];
+          var cover3 := cover1+cover2+{entryBlockId}+{thnExitId}+{elsExitId};
+
+          assert IsAcyclicAlt(successors, entryBlockId, cover3);
+          
+          //assert cover3 == CoveringSet(nextVersion, nextVersion2, {precedingBlock.0}, {nextVersion2});
+
+          assert IsAcyclicAlt(successors, entryBlockId, CoveringSet(nextVersion, nextVersion2+1, {precedingBlock.0}, {nextVersion2})) by {
+            assert cover3 == CoveringSet(nextVersion, nextVersion2+1, {precedingBlock.0}, {nextVersion2});
+          }
+        } else {
+          assume false;
+        }
     }
   }           
 
